coq/Field.v
@@ -1,4 +1,4 @@
-(* $Id: Field.v,v 1.10 2013-07-26 09:46:17 deraugla Exp $ *)
+(* $Id: Field.v,v 1.11 2013-07-26 18:16:10 deraugla Exp $ *)
 
 Require Import Utf8.
 
@@ -9,14 +9,9 @@ Record field α :=
     one : α;
     add : α → α → α;
     mul : α → α → α;
-    fld_eq : α → α → bool;
-    fld_eq_refl : ∀ a,
-      fld_eq a a = true;
-    fld_eq_sym : ∀ a b,
-      fld_eq a b = fld_eq b a;
-    fld_eq_trans : ∀ a b c,
-      fld_eq a b = true → fld_eq b c = true → fld_eq a c = true;
-    fld_add_comm : ∀ a b,
-      fld_eq (add a b) (add b a) = true;
-    fld_add_assoc : ∀ a b c,
-      fld_eq (add (add a b) c) (add a (add b c)) = true }.
+    fld_eq : α → α → Prop;
+    fld_eq_refl : ∀ a, fld_eq a a;
+    fld_eq_sym : ∀ a b, fld_eq a b → fld_eq b a;
+    fld_eq_trans : ∀ a b c, fld_eq a b → fld_eq b c → fld_eq a c;
+    fld_add_comm : ∀ a b, fld_eq (add a b) (add b a);
+    fld_add_assoc : ∀ a b c, fld_eq (add (add a b) c) (add a (add b c)) }.
